Add synthesis of relax
Now it makes sense, since we're using typedefs

fiat-c/src/p224_64.c
@@ -161,11 +161,6 @@ static void fiat_p224_cmovznz_u64(uint64_t* out1, fiat_p224_uint1 arg1, uint64_t
  *   eval (from_montgomery out1) mod m = (eval (from_montgomery arg1) * eval (from_montgomery arg2)) mod m
  *   0 ≤ eval out1 < m
  *
- * Input Bounds:
- *   arg1: [[0x0 ~> 0xffffffffffffffff], [0x0 ~> 0xffffffffffffffff], [0x0 ~> 0xffffffffffffffff], [0x0 ~> 0xffffffffffffffff]]
- *   arg2: [[0x0 ~> 0xffffffffffffffff], [0x0 ~> 0xffffffffffffffff], [0x0 ~> 0xffffffffffffffff], [0x0 ~> 0xffffffffffffffff]]
- * Output Bounds:
- *   out1: [[0x0 ~> 0xffffffffffffffff], [0x0 ~> 0xffffffffffffffff], [0x0 ~> 0xffffffffffffffff], [0x0 ~> 0xffffffffffffffff]]
  */
 static void fiat_p224_mul(fiat_p224_montgomery_domain_field_element out1, const fiat_p224_montgomery_domain_field_element arg1, const fiat_p224_montgomery_domain_field_element arg2) {
   uint64_t x1;
@@ -497,10 +492,6 @@ static void fiat_p224_mul(fiat_p224_montgomery_domain_field_element out1, const 
  *   eval (from_montgomery out1) mod m = (eval (from_montgomery arg1) * eval (from_montgomery arg1)) mod m
  *   0 ≤ eval out1 < m
  *
- * Input Bounds:
- *   arg1: [[0x0 ~> 0xffffffffffffffff], [0x0 ~> 0xffffffffffffffff], [0x0 ~> 0xffffffffffffffff], [0x0 ~> 0xffffffffffffffff]]
- * Output Bounds:
- *   out1: [[0x0 ~> 0xffffffffffffffff], [0x0 ~> 0xffffffffffffffff], [0x0 ~> 0xffffffffffffffff], [0x0 ~> 0xffffffffffffffff]]
  */
 static void fiat_p224_square(fiat_p224_montgomery_domain_field_element out1, const fiat_p224_montgomery_domain_field_element arg1) {
   uint64_t x1;
@@ -833,11 +824,6 @@ static void fiat_p224_square(fiat_p224_montgomery_domain_field_element out1, con
  *   eval (from_montgomery out1) mod m = (eval (from_montgomery arg1) + eval (from_montgomery arg2)) mod m
  *   0 ≤ eval out1 < m
  *
- * Input Bounds:
- *   arg1: [[0x0 ~> 0xffffffffffffffff], [0x0 ~> 0xffffffffffffffff], [0x0 ~> 0xffffffffffffffff], [0x0 ~> 0xffffffffffffffff]]
- *   arg2: [[0x0 ~> 0xffffffffffffffff], [0x0 ~> 0xffffffffffffffff], [0x0 ~> 0xffffffffffffffff], [0x0 ~> 0xffffffffffffffff]]
- * Output Bounds:
- *   out1: [[0x0 ~> 0xffffffffffffffff], [0x0 ~> 0xffffffffffffffff], [0x0 ~> 0xffffffffffffffff], [0x0 ~> 0xffffffffffffffff]]
  */
 static void fiat_p224_add(fiat_p224_montgomery_domain_field_element out1, const fiat_p224_montgomery_domain_field_element arg1, const fiat_p224_montgomery_domain_field_element arg2) {
   uint64_t x1;
@@ -891,11 +877,6 @@ static void fiat_p224_add(fiat_p224_montgomery_domain_field_element out1, const 
  *   eval (from_montgomery out1) mod m = (eval (from_montgomery arg1) - eval (from_montgomery arg2)) mod m
  *   0 ≤ eval out1 < m
  *
- * Input Bounds:
- *   arg1: [[0x0 ~> 0xffffffffffffffff], [0x0 ~> 0xffffffffffffffff], [0x0 ~> 0xffffffffffffffff], [0x0 ~> 0xffffffffffffffff]]
- *   arg2: [[0x0 ~> 0xffffffffffffffff], [0x0 ~> 0xffffffffffffffff], [0x0 ~> 0xffffffffffffffff], [0x0 ~> 0xffffffffffffffff]]
- * Output Bounds:
- *   out1: [[0x0 ~> 0xffffffffffffffff], [0x0 ~> 0xffffffffffffffff], [0x0 ~> 0xffffffffffffffff], [0x0 ~> 0xffffffffffffffff]]
  */
 static void fiat_p224_sub(fiat_p224_montgomery_domain_field_element out1, const fiat_p224_montgomery_domain_field_element arg1, const fiat_p224_montgomery_domain_field_element arg2) {
   uint64_t x1;
@@ -939,10 +920,6 @@ static void fiat_p224_sub(fiat_p224_montgomery_domain_field_element out1, const 
  *   eval (from_montgomery out1) mod m = -eval (from_montgomery arg1) mod m
  *   0 ≤ eval out1 < m
  *
- * Input Bounds:
- *   arg1: [[0x0 ~> 0xffffffffffffffff], [0x0 ~> 0xffffffffffffffff], [0x0 ~> 0xffffffffffffffff], [0x0 ~> 0xffffffffffffffff]]
- * Output Bounds:
- *   out1: [[0x0 ~> 0xffffffffffffffff], [0x0 ~> 0xffffffffffffffff], [0x0 ~> 0xffffffffffffffff], [0x0 ~> 0xffffffffffffffff]]
  */
 static void fiat_p224_opp(fiat_p224_montgomery_domain_field_element out1, const fiat_p224_montgomery_domain_field_element arg1) {
   uint64_t x1;
@@ -986,10 +963,6 @@ static void fiat_p224_opp(fiat_p224_montgomery_domain_field_element out1, const 
  *   eval out1 mod m = (eval arg1 * ((2^64)⁻¹ mod m)^4) mod m
  *   0 ≤ eval out1 < m
  *
- * Input Bounds:
- *   arg1: [[0x0 ~> 0xffffffffffffffff], [0x0 ~> 0xffffffffffffffff], [0x0 ~> 0xffffffffffffffff], [0x0 ~> 0xffffffffffffffff]]
- * Output Bounds:
- *   out1: [[0x0 ~> 0xffffffffffffffff], [0x0 ~> 0xffffffffffffffff], [0x0 ~> 0xffffffffffffffff], [0x0 ~> 0xffffffffffffffff]]
  */
 static void fiat_p224_from_montgomery(fiat_p224_non_montgomery_domain_field_element out1, const fiat_p224_montgomery_domain_field_element arg1) {
   uint64_t x1;
@@ -1181,10 +1154,6 @@ static void fiat_p224_from_montgomery(fiat_p224_non_montgomery_domain_field_elem
  *   eval (from_montgomery out1) mod m = eval arg1 mod m
  *   0 ≤ eval out1 < m
  *
- * Input Bounds:
- *   arg1: [[0x0 ~> 0xffffffffffffffff], [0x0 ~> 0xffffffffffffffff], [0x0 ~> 0xffffffffffffffff], [0x0 ~> 0xffffffffffffffff]]
- * Output Bounds:
- *   out1: [[0x0 ~> 0xffffffffffffffff], [0x0 ~> 0xffffffffffffffff], [0x0 ~> 0xffffffffffffffff], [0x0 ~> 0xffffffffffffffff]]
  */
 static void fiat_p224_to_montgomery(fiat_p224_montgomery_domain_field_element out1, const fiat_p224_non_montgomery_domain_field_element arg1) {
   uint64_t x1;
@@ -1793,8 +1762,6 @@ static void fiat_p224_from_bytes(uint64_t out1[4], const uint8_t arg1[28]) {
  *   eval (from_montgomery out1) mod m = 1 mod m
  *   0 ≤ eval out1 < m
  *
- * Output Bounds:
- *   out1: [[0x0 ~> 0xffffffffffffffff], [0x0 ~> 0xffffffffffffffff], [0x0 ~> 0xffffffffffffffff], [0x0 ~> 0xffffffffffffffff]]
  */
 static void fiat_p224_set_one(fiat_p224_montgomery_domain_field_element out1) {
   out1[0] = UINT64_C(0xffffffff00000000);
