fiat-c/src/p384_64.c
@@ -161,11 +161,6 @@ static void fiat_p384_cmovznz_u64(uint64_t* out1, fiat_p384_uint1 arg1, uint64_t
  *   eval (from_montgomery out1) mod m = (eval (from_montgomery arg1) * eval (from_montgomery arg2)) mod m
  *   0 ≤ eval out1 < m
  *
- * Input Bounds:
- *   arg1: [[0x0 ~> 0xffffffffffffffff], [0x0 ~> 0xffffffffffffffff], [0x0 ~> 0xffffffffffffffff], [0x0 ~> 0xffffffffffffffff], [0x0 ~> 0xffffffffffffffff], [0x0 ~> 0xffffffffffffffff]]
- *   arg2: [[0x0 ~> 0xffffffffffffffff], [0x0 ~> 0xffffffffffffffff], [0x0 ~> 0xffffffffffffffff], [0x0 ~> 0xffffffffffffffff], [0x0 ~> 0xffffffffffffffff], [0x0 ~> 0xffffffffffffffff]]
- * Output Bounds:
- *   out1: [[0x0 ~> 0xffffffffffffffff], [0x0 ~> 0xffffffffffffffff], [0x0 ~> 0xffffffffffffffff], [0x0 ~> 0xffffffffffffffff], [0x0 ~> 0xffffffffffffffff], [0x0 ~> 0xffffffffffffffff]]
  */
 static void fiat_p384_mul(fiat_p384_montgomery_domain_field_element out1, const fiat_p384_montgomery_domain_field_element arg1, const fiat_p384_montgomery_domain_field_element arg2) {
   uint64_t x1;
@@ -909,10 +904,6 @@ static void fiat_p384_mul(fiat_p384_montgomery_domain_field_element out1, const 
  *   eval (from_montgomery out1) mod m = (eval (from_montgomery arg1) * eval (from_montgomery arg1)) mod m
  *   0 ≤ eval out1 < m
  *
- * Input Bounds:
- *   arg1: [[0x0 ~> 0xffffffffffffffff], [0x0 ~> 0xffffffffffffffff], [0x0 ~> 0xffffffffffffffff], [0x0 ~> 0xffffffffffffffff], [0x0 ~> 0xffffffffffffffff], [0x0 ~> 0xffffffffffffffff]]
- * Output Bounds:
- *   out1: [[0x0 ~> 0xffffffffffffffff], [0x0 ~> 0xffffffffffffffff], [0x0 ~> 0xffffffffffffffff], [0x0 ~> 0xffffffffffffffff], [0x0 ~> 0xffffffffffffffff], [0x0 ~> 0xffffffffffffffff]]
  */
 static void fiat_p384_square(fiat_p384_montgomery_domain_field_element out1, const fiat_p384_montgomery_domain_field_element arg1) {
   uint64_t x1;
@@ -1657,11 +1648,6 @@ static void fiat_p384_square(fiat_p384_montgomery_domain_field_element out1, con
  *   eval (from_montgomery out1) mod m = (eval (from_montgomery arg1) + eval (from_montgomery arg2)) mod m
  *   0 ≤ eval out1 < m
  *
- * Input Bounds:
- *   arg1: [[0x0 ~> 0xffffffffffffffff], [0x0 ~> 0xffffffffffffffff], [0x0 ~> 0xffffffffffffffff], [0x0 ~> 0xffffffffffffffff], [0x0 ~> 0xffffffffffffffff], [0x0 ~> 0xffffffffffffffff]]
- *   arg2: [[0x0 ~> 0xffffffffffffffff], [0x0 ~> 0xffffffffffffffff], [0x0 ~> 0xffffffffffffffff], [0x0 ~> 0xffffffffffffffff], [0x0 ~> 0xffffffffffffffff], [0x0 ~> 0xffffffffffffffff]]
- * Output Bounds:
- *   out1: [[0x0 ~> 0xffffffffffffffff], [0x0 ~> 0xffffffffffffffff], [0x0 ~> 0xffffffffffffffff], [0x0 ~> 0xffffffffffffffff], [0x0 ~> 0xffffffffffffffff], [0x0 ~> 0xffffffffffffffff]]
  */
 static void fiat_p384_add(fiat_p384_montgomery_domain_field_element out1, const fiat_p384_montgomery_domain_field_element arg1, const fiat_p384_montgomery_domain_field_element arg2) {
   uint64_t x1;
@@ -1733,11 +1719,6 @@ static void fiat_p384_add(fiat_p384_montgomery_domain_field_element out1, const 
  *   eval (from_montgomery out1) mod m = (eval (from_montgomery arg1) - eval (from_montgomery arg2)) mod m
  *   0 ≤ eval out1 < m
  *
- * Input Bounds:
- *   arg1: [[0x0 ~> 0xffffffffffffffff], [0x0 ~> 0xffffffffffffffff], [0x0 ~> 0xffffffffffffffff], [0x0 ~> 0xffffffffffffffff], [0x0 ~> 0xffffffffffffffff], [0x0 ~> 0xffffffffffffffff]]
- *   arg2: [[0x0 ~> 0xffffffffffffffff], [0x0 ~> 0xffffffffffffffff], [0x0 ~> 0xffffffffffffffff], [0x0 ~> 0xffffffffffffffff], [0x0 ~> 0xffffffffffffffff], [0x0 ~> 0xffffffffffffffff]]
- * Output Bounds:
- *   out1: [[0x0 ~> 0xffffffffffffffff], [0x0 ~> 0xffffffffffffffff], [0x0 ~> 0xffffffffffffffff], [0x0 ~> 0xffffffffffffffff], [0x0 ~> 0xffffffffffffffff], [0x0 ~> 0xffffffffffffffff]]
  */
 static void fiat_p384_sub(fiat_p384_montgomery_domain_field_element out1, const fiat_p384_montgomery_domain_field_element arg1, const fiat_p384_montgomery_domain_field_element arg2) {
   uint64_t x1;
@@ -1795,10 +1776,6 @@ static void fiat_p384_sub(fiat_p384_montgomery_domain_field_element out1, const 
  *   eval (from_montgomery out1) mod m = -eval (from_montgomery arg1) mod m
  *   0 ≤ eval out1 < m
  *
- * Input Bounds:
- *   arg1: [[0x0 ~> 0xffffffffffffffff], [0x0 ~> 0xffffffffffffffff], [0x0 ~> 0xffffffffffffffff], [0x0 ~> 0xffffffffffffffff], [0x0 ~> 0xffffffffffffffff], [0x0 ~> 0xffffffffffffffff]]
- * Output Bounds:
- *   out1: [[0x0 ~> 0xffffffffffffffff], [0x0 ~> 0xffffffffffffffff], [0x0 ~> 0xffffffffffffffff], [0x0 ~> 0xffffffffffffffff], [0x0 ~> 0xffffffffffffffff], [0x0 ~> 0xffffffffffffffff]]
  */
 static void fiat_p384_opp(fiat_p384_montgomery_domain_field_element out1, const fiat_p384_montgomery_domain_field_element arg1) {
   uint64_t x1;
@@ -1856,10 +1833,6 @@ static void fiat_p384_opp(fiat_p384_montgomery_domain_field_element out1, const 
  *   eval out1 mod m = (eval arg1 * ((2^64)⁻¹ mod m)^6) mod m
  *   0 ≤ eval out1 < m
  *
- * Input Bounds:
- *   arg1: [[0x0 ~> 0xffffffffffffffff], [0x0 ~> 0xffffffffffffffff], [0x0 ~> 0xffffffffffffffff], [0x0 ~> 0xffffffffffffffff], [0x0 ~> 0xffffffffffffffff], [0x0 ~> 0xffffffffffffffff]]
- * Output Bounds:
- *   out1: [[0x0 ~> 0xffffffffffffffff], [0x0 ~> 0xffffffffffffffff], [0x0 ~> 0xffffffffffffffff], [0x0 ~> 0xffffffffffffffff], [0x0 ~> 0xffffffffffffffff], [0x0 ~> 0xffffffffffffffff]]
  */
 static void fiat_p384_from_montgomery(fiat_p384_non_montgomery_domain_field_element out1, const fiat_p384_montgomery_domain_field_element arg1) {
   uint64_t x1;
@@ -2346,10 +2319,6 @@ static void fiat_p384_from_montgomery(fiat_p384_non_montgomery_domain_field_elem
  *   eval (from_montgomery out1) mod m = eval arg1 mod m
  *   0 ≤ eval out1 < m
  *
- * Input Bounds:
- *   arg1: [[0x0 ~> 0xffffffffffffffff], [0x0 ~> 0xffffffffffffffff], [0x0 ~> 0xffffffffffffffff], [0x0 ~> 0xffffffffffffffff], [0x0 ~> 0xffffffffffffffff], [0x0 ~> 0xffffffffffffffff]]
- * Output Bounds:
- *   out1: [[0x0 ~> 0xffffffffffffffff], [0x0 ~> 0xffffffffffffffff], [0x0 ~> 0xffffffffffffffff], [0x0 ~> 0xffffffffffffffff], [0x0 ~> 0xffffffffffffffff], [0x0 ~> 0xffffffffffffffff]]
  */
 static void fiat_p384_to_montgomery(fiat_p384_montgomery_domain_field_element out1, const fiat_p384_non_montgomery_domain_field_element arg1) {
   uint64_t x1;
@@ -3488,8 +3457,6 @@ static void fiat_p384_from_bytes(uint64_t out1[6], const uint8_t arg1[48]) {
  *   eval (from_montgomery out1) mod m = 1 mod m
  *   0 ≤ eval out1 < m
  *
- * Output Bounds:
- *   out1: [[0x0 ~> 0xffffffffffffffff], [0x0 ~> 0xffffffffffffffff], [0x0 ~> 0xffffffffffffffff], [0x0 ~> 0xffffffffffffffff], [0x0 ~> 0xffffffffffffffff], [0x0 ~> 0xffffffffffffffff]]
  */
 static void fiat_p384_set_one(fiat_p384_montgomery_domain_field_element out1) {
   out1[0] = UINT64_C(0xffffffff00000001);
