fiat-go/32/p256/p256.go
@@ -90,11 +90,6 @@ func cmovznzU32(out1 *uint32, arg1 uint1, arg2 uint32, arg3 uint32) {
 //   eval (from_montgomery out1) mod m = (eval (from_montgomery arg1) * eval (from_montgomery arg2)) mod m
 //   0 ≤ eval out1 < m
 //
-// Input Bounds:
-//   arg1: [[0x0 ~> 0xffffffff], [0x0 ~> 0xffffffff], [0x0 ~> 0xffffffff], [0x0 ~> 0xffffffff], [0x0 ~> 0xffffffff], [0x0 ~> 0xffffffff], [0x0 ~> 0xffffffff], [0x0 ~> 0xffffffff]]
-//   arg2: [[0x0 ~> 0xffffffff], [0x0 ~> 0xffffffff], [0x0 ~> 0xffffffff], [0x0 ~> 0xffffffff], [0x0 ~> 0xffffffff], [0x0 ~> 0xffffffff], [0x0 ~> 0xffffffff], [0x0 ~> 0xffffffff]]
-// Output Bounds:
-//   out1: [[0x0 ~> 0xffffffff], [0x0 ~> 0xffffffff], [0x0 ~> 0xffffffff], [0x0 ~> 0xffffffff], [0x0 ~> 0xffffffff], [0x0 ~> 0xffffffff], [0x0 ~> 0xffffffff], [0x0 ~> 0xffffffff]]
 func Mul(out1 *MontgomeryDomainFieldElement, arg1 *MontgomeryDomainFieldElement, arg2 *MontgomeryDomainFieldElement) {
 	x1 := arg1[1]
 	x2 := arg1[2]
@@ -1088,10 +1083,6 @@ func Mul(out1 *MontgomeryDomainFieldElement, arg1 *MontgomeryDomainFieldElement,
 //   eval (from_montgomery out1) mod m = (eval (from_montgomery arg1) * eval (from_montgomery arg1)) mod m
 //   0 ≤ eval out1 < m
 //
-// Input Bounds:
-//   arg1: [[0x0 ~> 0xffffffff], [0x0 ~> 0xffffffff], [0x0 ~> 0xffffffff], [0x0 ~> 0xffffffff], [0x0 ~> 0xffffffff], [0x0 ~> 0xffffffff], [0x0 ~> 0xffffffff], [0x0 ~> 0xffffffff]]
-// Output Bounds:
-//   out1: [[0x0 ~> 0xffffffff], [0x0 ~> 0xffffffff], [0x0 ~> 0xffffffff], [0x0 ~> 0xffffffff], [0x0 ~> 0xffffffff], [0x0 ~> 0xffffffff], [0x0 ~> 0xffffffff], [0x0 ~> 0xffffffff]]
 func Square(out1 *MontgomeryDomainFieldElement, arg1 *MontgomeryDomainFieldElement) {
 	x1 := arg1[1]
 	x2 := arg1[2]
@@ -2086,11 +2077,6 @@ func Square(out1 *MontgomeryDomainFieldElement, arg1 *MontgomeryDomainFieldEleme
 //   eval (from_montgomery out1) mod m = (eval (from_montgomery arg1) + eval (from_montgomery arg2)) mod m
 //   0 ≤ eval out1 < m
 //
-// Input Bounds:
-//   arg1: [[0x0 ~> 0xffffffff], [0x0 ~> 0xffffffff], [0x0 ~> 0xffffffff], [0x0 ~> 0xffffffff], [0x0 ~> 0xffffffff], [0x0 ~> 0xffffffff], [0x0 ~> 0xffffffff], [0x0 ~> 0xffffffff]]
-//   arg2: [[0x0 ~> 0xffffffff], [0x0 ~> 0xffffffff], [0x0 ~> 0xffffffff], [0x0 ~> 0xffffffff], [0x0 ~> 0xffffffff], [0x0 ~> 0xffffffff], [0x0 ~> 0xffffffff], [0x0 ~> 0xffffffff]]
-// Output Bounds:
-//   out1: [[0x0 ~> 0xffffffff], [0x0 ~> 0xffffffff], [0x0 ~> 0xffffffff], [0x0 ~> 0xffffffff], [0x0 ~> 0xffffffff], [0x0 ~> 0xffffffff], [0x0 ~> 0xffffffff], [0x0 ~> 0xffffffff]]
 func Add(out1 *MontgomeryDomainFieldElement, arg1 *MontgomeryDomainFieldElement, arg2 *MontgomeryDomainFieldElement) {
 	var x1 uint32
 	var x2 uint1
@@ -2177,11 +2163,6 @@ func Add(out1 *MontgomeryDomainFieldElement, arg1 *MontgomeryDomainFieldElement,
 //   eval (from_montgomery out1) mod m = (eval (from_montgomery arg1) - eval (from_montgomery arg2)) mod m
 //   0 ≤ eval out1 < m
 //
-// Input Bounds:
-//   arg1: [[0x0 ~> 0xffffffff], [0x0 ~> 0xffffffff], [0x0 ~> 0xffffffff], [0x0 ~> 0xffffffff], [0x0 ~> 0xffffffff], [0x0 ~> 0xffffffff], [0x0 ~> 0xffffffff], [0x0 ~> 0xffffffff]]
-//   arg2: [[0x0 ~> 0xffffffff], [0x0 ~> 0xffffffff], [0x0 ~> 0xffffffff], [0x0 ~> 0xffffffff], [0x0 ~> 0xffffffff], [0x0 ~> 0xffffffff], [0x0 ~> 0xffffffff], [0x0 ~> 0xffffffff]]
-// Output Bounds:
-//   out1: [[0x0 ~> 0xffffffff], [0x0 ~> 0xffffffff], [0x0 ~> 0xffffffff], [0x0 ~> 0xffffffff], [0x0 ~> 0xffffffff], [0x0 ~> 0xffffffff], [0x0 ~> 0xffffffff], [0x0 ~> 0xffffffff]]
 func Sub(out1 *MontgomeryDomainFieldElement, arg1 *MontgomeryDomainFieldElement, arg2 *MontgomeryDomainFieldElement) {
 	var x1 uint32
 	var x2 uint1
@@ -2250,10 +2231,6 @@ func Sub(out1 *MontgomeryDomainFieldElement, arg1 *MontgomeryDomainFieldElement,
 //   eval (from_montgomery out1) mod m = -eval (from_montgomery arg1) mod m
 //   0 ≤ eval out1 < m
 //
-// Input Bounds:
-//   arg1: [[0x0 ~> 0xffffffff], [0x0 ~> 0xffffffff], [0x0 ~> 0xffffffff], [0x0 ~> 0xffffffff], [0x0 ~> 0xffffffff], [0x0 ~> 0xffffffff], [0x0 ~> 0xffffffff], [0x0 ~> 0xffffffff]]
-// Output Bounds:
-//   out1: [[0x0 ~> 0xffffffff], [0x0 ~> 0xffffffff], [0x0 ~> 0xffffffff], [0x0 ~> 0xffffffff], [0x0 ~> 0xffffffff], [0x0 ~> 0xffffffff], [0x0 ~> 0xffffffff], [0x0 ~> 0xffffffff]]
 func Opp(out1 *MontgomeryDomainFieldElement, arg1 *MontgomeryDomainFieldElement) {
 	var x1 uint32
 	var x2 uint1
@@ -2322,10 +2299,6 @@ func Opp(out1 *MontgomeryDomainFieldElement, arg1 *MontgomeryDomainFieldElement)
 //   eval out1 mod m = (eval arg1 * ((2^32)⁻¹ mod m)^8) mod m
 //   0 ≤ eval out1 < m
 //
-// Input Bounds:
-//   arg1: [[0x0 ~> 0xffffffff], [0x0 ~> 0xffffffff], [0x0 ~> 0xffffffff], [0x0 ~> 0xffffffff], [0x0 ~> 0xffffffff], [0x0 ~> 0xffffffff], [0x0 ~> 0xffffffff], [0x0 ~> 0xffffffff]]
-// Output Bounds:
-//   out1: [[0x0 ~> 0xffffffff], [0x0 ~> 0xffffffff], [0x0 ~> 0xffffffff], [0x0 ~> 0xffffffff], [0x0 ~> 0xffffffff], [0x0 ~> 0xffffffff], [0x0 ~> 0xffffffff], [0x0 ~> 0xffffffff]]
 func FromMontgomery(out1 *NonMontgomeryDomainFieldElement, arg1 *MontgomeryDomainFieldElement) {
 	x1 := arg1[0]
 	var x2 uint32
@@ -2851,10 +2824,6 @@ func FromMontgomery(out1 *NonMontgomeryDomainFieldElement, arg1 *MontgomeryDomai
 //   eval (from_montgomery out1) mod m = eval arg1 mod m
 //   0 ≤ eval out1 < m
 //
-// Input Bounds:
-//   arg1: [[0x0 ~> 0xffffffff], [0x0 ~> 0xffffffff], [0x0 ~> 0xffffffff], [0x0 ~> 0xffffffff], [0x0 ~> 0xffffffff], [0x0 ~> 0xffffffff], [0x0 ~> 0xffffffff], [0x0 ~> 0xffffffff]]
-// Output Bounds:
-//   out1: [[0x0 ~> 0xffffffff], [0x0 ~> 0xffffffff], [0x0 ~> 0xffffffff], [0x0 ~> 0xffffffff], [0x0 ~> 0xffffffff], [0x0 ~> 0xffffffff], [0x0 ~> 0xffffffff], [0x0 ~> 0xffffffff]]
 func ToMontgomery(out1 *MontgomeryDomainFieldElement, arg1 *NonMontgomeryDomainFieldElement) {
 	x1 := arg1[1]
 	x2 := arg1[2]
@@ -3965,8 +3934,6 @@ func FromBytes(out1 *[8]uint32, arg1 *[32]uint8) {
 //   eval (from_montgomery out1) mod m = 1 mod m
 //   0 ≤ eval out1 < m
 //
-// Output Bounds:
-//   out1: [[0x0 ~> 0xffffffff], [0x0 ~> 0xffffffff], [0x0 ~> 0xffffffff], [0x0 ~> 0xffffffff], [0x0 ~> 0xffffffff], [0x0 ~> 0xffffffff], [0x0 ~> 0xffffffff], [0x0 ~> 0xffffffff]]
 func SetOne(out1 *MontgomeryDomainFieldElement) {
 	out1[0] = uint32(0x1)
 	out1[1] = uint32(0x0)
