fiat-rust/src/p256_32.rs
@@ -127,11 +127,6 @@ pub fn fiat_p256_cmovznz_u32(out1: &mut u32, arg1: fiat_p256_u1, arg2: u32, arg3
 ///   eval (from_montgomery out1) mod m = (eval (from_montgomery arg1) * eval (from_montgomery arg2)) mod m
 ///   0 ≤ eval out1 < m
 ///
-/// Input Bounds:
-///   arg1: [[0x0 ~> 0xffffffff], [0x0 ~> 0xffffffff], [0x0 ~> 0xffffffff], [0x0 ~> 0xffffffff], [0x0 ~> 0xffffffff], [0x0 ~> 0xffffffff], [0x0 ~> 0xffffffff], [0x0 ~> 0xffffffff]]
-///   arg2: [[0x0 ~> 0xffffffff], [0x0 ~> 0xffffffff], [0x0 ~> 0xffffffff], [0x0 ~> 0xffffffff], [0x0 ~> 0xffffffff], [0x0 ~> 0xffffffff], [0x0 ~> 0xffffffff], [0x0 ~> 0xffffffff]]
-/// Output Bounds:
-///   out1: [[0x0 ~> 0xffffffff], [0x0 ~> 0xffffffff], [0x0 ~> 0xffffffff], [0x0 ~> 0xffffffff], [0x0 ~> 0xffffffff], [0x0 ~> 0xffffffff], [0x0 ~> 0xffffffff], [0x0 ~> 0xffffffff]]
 #[inline]
 pub fn fiat_p256_mul(out1: &mut fiat_p256_montgomery_domain_field_element, arg1: &fiat_p256_montgomery_domain_field_element, arg2: &fiat_p256_montgomery_domain_field_element) -> () {
   let x1: u32 = (arg1[1]);
@@ -1135,10 +1130,6 @@ pub fn fiat_p256_mul(out1: &mut fiat_p256_montgomery_domain_field_element, arg1:
 ///   eval (from_montgomery out1) mod m = (eval (from_montgomery arg1) * eval (from_montgomery arg1)) mod m
 ///   0 ≤ eval out1 < m
 ///
-/// Input Bounds:
-///   arg1: [[0x0 ~> 0xffffffff], [0x0 ~> 0xffffffff], [0x0 ~> 0xffffffff], [0x0 ~> 0xffffffff], [0x0 ~> 0xffffffff], [0x0 ~> 0xffffffff], [0x0 ~> 0xffffffff], [0x0 ~> 0xffffffff]]
-/// Output Bounds:
-///   out1: [[0x0 ~> 0xffffffff], [0x0 ~> 0xffffffff], [0x0 ~> 0xffffffff], [0x0 ~> 0xffffffff], [0x0 ~> 0xffffffff], [0x0 ~> 0xffffffff], [0x0 ~> 0xffffffff], [0x0 ~> 0xffffffff]]
 #[inline]
 pub fn fiat_p256_square(out1: &mut fiat_p256_montgomery_domain_field_element, arg1: &fiat_p256_montgomery_domain_field_element) -> () {
   let x1: u32 = (arg1[1]);
@@ -2143,11 +2134,6 @@ pub fn fiat_p256_square(out1: &mut fiat_p256_montgomery_domain_field_element, ar
 ///   eval (from_montgomery out1) mod m = (eval (from_montgomery arg1) + eval (from_montgomery arg2)) mod m
 ///   0 ≤ eval out1 < m
 ///
-/// Input Bounds:
-///   arg1: [[0x0 ~> 0xffffffff], [0x0 ~> 0xffffffff], [0x0 ~> 0xffffffff], [0x0 ~> 0xffffffff], [0x0 ~> 0xffffffff], [0x0 ~> 0xffffffff], [0x0 ~> 0xffffffff], [0x0 ~> 0xffffffff]]
-///   arg2: [[0x0 ~> 0xffffffff], [0x0 ~> 0xffffffff], [0x0 ~> 0xffffffff], [0x0 ~> 0xffffffff], [0x0 ~> 0xffffffff], [0x0 ~> 0xffffffff], [0x0 ~> 0xffffffff], [0x0 ~> 0xffffffff]]
-/// Output Bounds:
-///   out1: [[0x0 ~> 0xffffffff], [0x0 ~> 0xffffffff], [0x0 ~> 0xffffffff], [0x0 ~> 0xffffffff], [0x0 ~> 0xffffffff], [0x0 ~> 0xffffffff], [0x0 ~> 0xffffffff], [0x0 ~> 0xffffffff]]
 #[inline]
 pub fn fiat_p256_add(out1: &mut fiat_p256_montgomery_domain_field_element, arg1: &fiat_p256_montgomery_domain_field_element, arg2: &fiat_p256_montgomery_domain_field_element) -> () {
   let mut x1: u32 = 0;
@@ -2236,11 +2222,6 @@ pub fn fiat_p256_add(out1: &mut fiat_p256_montgomery_domain_field_element, arg1:
 ///   eval (from_montgomery out1) mod m = (eval (from_montgomery arg1) - eval (from_montgomery arg2)) mod m
 ///   0 ≤ eval out1 < m
 ///
-/// Input Bounds:
-///   arg1: [[0x0 ~> 0xffffffff], [0x0 ~> 0xffffffff], [0x0 ~> 0xffffffff], [0x0 ~> 0xffffffff], [0x0 ~> 0xffffffff], [0x0 ~> 0xffffffff], [0x0 ~> 0xffffffff], [0x0 ~> 0xffffffff]]
-///   arg2: [[0x0 ~> 0xffffffff], [0x0 ~> 0xffffffff], [0x0 ~> 0xffffffff], [0x0 ~> 0xffffffff], [0x0 ~> 0xffffffff], [0x0 ~> 0xffffffff], [0x0 ~> 0xffffffff], [0x0 ~> 0xffffffff]]
-/// Output Bounds:
-///   out1: [[0x0 ~> 0xffffffff], [0x0 ~> 0xffffffff], [0x0 ~> 0xffffffff], [0x0 ~> 0xffffffff], [0x0 ~> 0xffffffff], [0x0 ~> 0xffffffff], [0x0 ~> 0xffffffff], [0x0 ~> 0xffffffff]]
 #[inline]
 pub fn fiat_p256_sub(out1: &mut fiat_p256_montgomery_domain_field_element, arg1: &fiat_p256_montgomery_domain_field_element, arg2: &fiat_p256_montgomery_domain_field_element) -> () {
   let mut x1: u32 = 0;
@@ -2311,10 +2292,6 @@ pub fn fiat_p256_sub(out1: &mut fiat_p256_montgomery_domain_field_element, arg1:
 ///   eval (from_montgomery out1) mod m = -eval (from_montgomery arg1) mod m
 ///   0 ≤ eval out1 < m
 ///
-/// Input Bounds:
-///   arg1: [[0x0 ~> 0xffffffff], [0x0 ~> 0xffffffff], [0x0 ~> 0xffffffff], [0x0 ~> 0xffffffff], [0x0 ~> 0xffffffff], [0x0 ~> 0xffffffff], [0x0 ~> 0xffffffff], [0x0 ~> 0xffffffff]]
-/// Output Bounds:
-///   out1: [[0x0 ~> 0xffffffff], [0x0 ~> 0xffffffff], [0x0 ~> 0xffffffff], [0x0 ~> 0xffffffff], [0x0 ~> 0xffffffff], [0x0 ~> 0xffffffff], [0x0 ~> 0xffffffff], [0x0 ~> 0xffffffff]]
 #[inline]
 pub fn fiat_p256_opp(out1: &mut fiat_p256_montgomery_domain_field_element, arg1: &fiat_p256_montgomery_domain_field_element) -> () {
   let mut x1: u32 = 0;
@@ -2385,10 +2362,6 @@ pub fn fiat_p256_opp(out1: &mut fiat_p256_montgomery_domain_field_element, arg1:
 ///   eval out1 mod m = (eval arg1 * ((2^32)⁻¹ mod m)^8) mod m
 ///   0 ≤ eval out1 < m
 ///
-/// Input Bounds:
-///   arg1: [[0x0 ~> 0xffffffff], [0x0 ~> 0xffffffff], [0x0 ~> 0xffffffff], [0x0 ~> 0xffffffff], [0x0 ~> 0xffffffff], [0x0 ~> 0xffffffff], [0x0 ~> 0xffffffff], [0x0 ~> 0xffffffff]]
-/// Output Bounds:
-///   out1: [[0x0 ~> 0xffffffff], [0x0 ~> 0xffffffff], [0x0 ~> 0xffffffff], [0x0 ~> 0xffffffff], [0x0 ~> 0xffffffff], [0x0 ~> 0xffffffff], [0x0 ~> 0xffffffff], [0x0 ~> 0xffffffff]]
 #[inline]
 pub fn fiat_p256_from_montgomery(out1: &mut fiat_p256_non_montgomery_domain_field_element, arg1: &fiat_p256_montgomery_domain_field_element) -> () {
   let x1: u32 = (arg1[0]);
@@ -2924,10 +2897,6 @@ pub fn fiat_p256_from_montgomery(out1: &mut fiat_p256_non_montgomery_domain_fiel
 ///   eval (from_montgomery out1) mod m = eval arg1 mod m
 ///   0 ≤ eval out1 < m
 ///
-/// Input Bounds:
-///   arg1: [[0x0 ~> 0xffffffff], [0x0 ~> 0xffffffff], [0x0 ~> 0xffffffff], [0x0 ~> 0xffffffff], [0x0 ~> 0xffffffff], [0x0 ~> 0xffffffff], [0x0 ~> 0xffffffff], [0x0 ~> 0xffffffff]]
-/// Output Bounds:
-///   out1: [[0x0 ~> 0xffffffff], [0x0 ~> 0xffffffff], [0x0 ~> 0xffffffff], [0x0 ~> 0xffffffff], [0x0 ~> 0xffffffff], [0x0 ~> 0xffffffff], [0x0 ~> 0xffffffff], [0x0 ~> 0xffffffff]]
 #[inline]
 pub fn fiat_p256_to_montgomery(out1: &mut fiat_p256_montgomery_domain_field_element, arg1: &fiat_p256_non_montgomery_domain_field_element) -> () {
   let x1: u32 = (arg1[1]);
@@ -4052,8 +4021,6 @@ pub fn fiat_p256_from_bytes(out1: &mut [u32; 8], arg1: &[u8; 32]) -> () {
 ///   eval (from_montgomery out1) mod m = 1 mod m
 ///   0 ≤ eval out1 < m
 ///
-/// Output Bounds:
-///   out1: [[0x0 ~> 0xffffffff], [0x0 ~> 0xffffffff], [0x0 ~> 0xffffffff], [0x0 ~> 0xffffffff], [0x0 ~> 0xffffffff], [0x0 ~> 0xffffffff], [0x0 ~> 0xffffffff], [0x0 ~> 0xffffffff]]
 #[inline]
 pub fn fiat_p256_set_one(out1: &mut fiat_p256_montgomery_domain_field_element) -> () {
   out1[0] = (0x1 as u32);
