fiat-rust/src/p256_64.rs
@@ -127,11 +127,6 @@ pub fn fiat_p256_cmovznz_u64(out1: &mut u64, arg1: fiat_p256_u1, arg2: u64, arg3
 ///   eval (from_montgomery out1) mod m = (eval (from_montgomery arg1) * eval (from_montgomery arg2)) mod m
 ///   0 ≤ eval out1 < m
 ///
-/// Input Bounds:
-///   arg1: [[0x0 ~> 0xffffffffffffffff], [0x0 ~> 0xffffffffffffffff], [0x0 ~> 0xffffffffffffffff], [0x0 ~> 0xffffffffffffffff]]
-///   arg2: [[0x0 ~> 0xffffffffffffffff], [0x0 ~> 0xffffffffffffffff], [0x0 ~> 0xffffffffffffffff], [0x0 ~> 0xffffffffffffffff]]
-/// Output Bounds:
-///   out1: [[0x0 ~> 0xffffffffffffffff], [0x0 ~> 0xffffffffffffffff], [0x0 ~> 0xffffffffffffffff], [0x0 ~> 0xffffffffffffffff]]
 #[inline]
 pub fn fiat_p256_mul(out1: &mut fiat_p256_montgomery_domain_field_element, arg1: &fiat_p256_montgomery_domain_field_element, arg2: &fiat_p256_montgomery_domain_field_element) -> () {
   let x1: u64 = (arg1[1]);
@@ -423,10 +418,6 @@ pub fn fiat_p256_mul(out1: &mut fiat_p256_montgomery_domain_field_element, arg1:
 ///   eval (from_montgomery out1) mod m = (eval (from_montgomery arg1) * eval (from_montgomery arg1)) mod m
 ///   0 ≤ eval out1 < m
 ///
-/// Input Bounds:
-///   arg1: [[0x0 ~> 0xffffffffffffffff], [0x0 ~> 0xffffffffffffffff], [0x0 ~> 0xffffffffffffffff], [0x0 ~> 0xffffffffffffffff]]
-/// Output Bounds:
-///   out1: [[0x0 ~> 0xffffffffffffffff], [0x0 ~> 0xffffffffffffffff], [0x0 ~> 0xffffffffffffffff], [0x0 ~> 0xffffffffffffffff]]
 #[inline]
 pub fn fiat_p256_square(out1: &mut fiat_p256_montgomery_domain_field_element, arg1: &fiat_p256_montgomery_domain_field_element) -> () {
   let x1: u64 = (arg1[1]);
@@ -719,11 +710,6 @@ pub fn fiat_p256_square(out1: &mut fiat_p256_montgomery_domain_field_element, ar
 ///   eval (from_montgomery out1) mod m = (eval (from_montgomery arg1) + eval (from_montgomery arg2)) mod m
 ///   0 ≤ eval out1 < m
 ///
-/// Input Bounds:
-///   arg1: [[0x0 ~> 0xffffffffffffffff], [0x0 ~> 0xffffffffffffffff], [0x0 ~> 0xffffffffffffffff], [0x0 ~> 0xffffffffffffffff]]
-///   arg2: [[0x0 ~> 0xffffffffffffffff], [0x0 ~> 0xffffffffffffffff], [0x0 ~> 0xffffffffffffffff], [0x0 ~> 0xffffffffffffffff]]
-/// Output Bounds:
-///   out1: [[0x0 ~> 0xffffffffffffffff], [0x0 ~> 0xffffffffffffffff], [0x0 ~> 0xffffffffffffffff], [0x0 ~> 0xffffffffffffffff]]
 #[inline]
 pub fn fiat_p256_add(out1: &mut fiat_p256_montgomery_domain_field_element, arg1: &fiat_p256_montgomery_domain_field_element, arg2: &fiat_p256_montgomery_domain_field_element) -> () {
   let mut x1: u64 = 0;
@@ -776,11 +762,6 @@ pub fn fiat_p256_add(out1: &mut fiat_p256_montgomery_domain_field_element, arg1:
 ///   eval (from_montgomery out1) mod m = (eval (from_montgomery arg1) - eval (from_montgomery arg2)) mod m
 ///   0 ≤ eval out1 < m
 ///
-/// Input Bounds:
-///   arg1: [[0x0 ~> 0xffffffffffffffff], [0x0 ~> 0xffffffffffffffff], [0x0 ~> 0xffffffffffffffff], [0x0 ~> 0xffffffffffffffff]]
-///   arg2: [[0x0 ~> 0xffffffffffffffff], [0x0 ~> 0xffffffffffffffff], [0x0 ~> 0xffffffffffffffff], [0x0 ~> 0xffffffffffffffff]]
-/// Output Bounds:
-///   out1: [[0x0 ~> 0xffffffffffffffff], [0x0 ~> 0xffffffffffffffff], [0x0 ~> 0xffffffffffffffff], [0x0 ~> 0xffffffffffffffff]]
 #[inline]
 pub fn fiat_p256_sub(out1: &mut fiat_p256_montgomery_domain_field_element, arg1: &fiat_p256_montgomery_domain_field_element, arg2: &fiat_p256_montgomery_domain_field_element) -> () {
   let mut x1: u64 = 0;
@@ -823,10 +804,6 @@ pub fn fiat_p256_sub(out1: &mut fiat_p256_montgomery_domain_field_element, arg1:
 ///   eval (from_montgomery out1) mod m = -eval (from_montgomery arg1) mod m
 ///   0 ≤ eval out1 < m
 ///
-/// Input Bounds:
-///   arg1: [[0x0 ~> 0xffffffffffffffff], [0x0 ~> 0xffffffffffffffff], [0x0 ~> 0xffffffffffffffff], [0x0 ~> 0xffffffffffffffff]]
-/// Output Bounds:
-///   out1: [[0x0 ~> 0xffffffffffffffff], [0x0 ~> 0xffffffffffffffff], [0x0 ~> 0xffffffffffffffff], [0x0 ~> 0xffffffffffffffff]]
 #[inline]
 pub fn fiat_p256_opp(out1: &mut fiat_p256_montgomery_domain_field_element, arg1: &fiat_p256_montgomery_domain_field_element) -> () {
   let mut x1: u64 = 0;
@@ -869,10 +846,6 @@ pub fn fiat_p256_opp(out1: &mut fiat_p256_montgomery_domain_field_element, arg1:
 ///   eval out1 mod m = (eval arg1 * ((2^64)⁻¹ mod m)^4) mod m
 ///   0 ≤ eval out1 < m
 ///
-/// Input Bounds:
-///   arg1: [[0x0 ~> 0xffffffffffffffff], [0x0 ~> 0xffffffffffffffff], [0x0 ~> 0xffffffffffffffff], [0x0 ~> 0xffffffffffffffff]]
-/// Output Bounds:
-///   out1: [[0x0 ~> 0xffffffffffffffff], [0x0 ~> 0xffffffffffffffff], [0x0 ~> 0xffffffffffffffff], [0x0 ~> 0xffffffffffffffff]]
 #[inline]
 pub fn fiat_p256_from_montgomery(out1: &mut fiat_p256_non_montgomery_domain_field_element, arg1: &fiat_p256_montgomery_domain_field_element) -> () {
   let x1: u64 = (arg1[0]);
@@ -1025,10 +998,6 @@ pub fn fiat_p256_from_montgomery(out1: &mut fiat_p256_non_montgomery_domain_fiel
 ///   eval (from_montgomery out1) mod m = eval arg1 mod m
 ///   0 ≤ eval out1 < m
 ///
-/// Input Bounds:
-///   arg1: [[0x0 ~> 0xffffffffffffffff], [0x0 ~> 0xffffffffffffffff], [0x0 ~> 0xffffffffffffffff], [0x0 ~> 0xffffffffffffffff]]
-/// Output Bounds:
-///   out1: [[0x0 ~> 0xffffffffffffffff], [0x0 ~> 0xffffffffffffffff], [0x0 ~> 0xffffffffffffffff], [0x0 ~> 0xffffffffffffffff]]
 #[inline]
 pub fn fiat_p256_to_montgomery(out1: &mut fiat_p256_montgomery_domain_field_element, arg1: &fiat_p256_non_montgomery_domain_field_element) -> () {
   let x1: u64 = (arg1[1]);
@@ -1529,8 +1498,6 @@ pub fn fiat_p256_from_bytes(out1: &mut [u64; 4], arg1: &[u8; 32]) -> () {
 ///   eval (from_montgomery out1) mod m = 1 mod m
 ///   0 ≤ eval out1 < m
 ///
-/// Output Bounds:
-///   out1: [[0x0 ~> 0xffffffffffffffff], [0x0 ~> 0xffffffffffffffff], [0x0 ~> 0xffffffffffffffff], [0x0 ~> 0xffffffffffffffff]]
 #[inline]
 pub fn fiat_p256_set_one(out1: &mut fiat_p256_montgomery_domain_field_element) -> () {
   out1[0] = (0x1 as u64);
