fiat-rust/src/p384_64.rs
@@ -127,11 +127,6 @@ pub fn fiat_p384_cmovznz_u64(out1: &mut u64, arg1: fiat_p384_u1, arg2: u64, arg3
 ///   eval (from_montgomery out1) mod m = (eval (from_montgomery arg1) * eval (from_montgomery arg2)) mod m
 ///   0 ≤ eval out1 < m
 ///
-/// Input Bounds:
-///   arg1: [[0x0 ~> 0xffffffffffffffff], [0x0 ~> 0xffffffffffffffff], [0x0 ~> 0xffffffffffffffff], [0x0 ~> 0xffffffffffffffff], [0x0 ~> 0xffffffffffffffff], [0x0 ~> 0xffffffffffffffff]]
-///   arg2: [[0x0 ~> 0xffffffffffffffff], [0x0 ~> 0xffffffffffffffff], [0x0 ~> 0xffffffffffffffff], [0x0 ~> 0xffffffffffffffff], [0x0 ~> 0xffffffffffffffff], [0x0 ~> 0xffffffffffffffff]]
-/// Output Bounds:
-///   out1: [[0x0 ~> 0xffffffffffffffff], [0x0 ~> 0xffffffffffffffff], [0x0 ~> 0xffffffffffffffff], [0x0 ~> 0xffffffffffffffff], [0x0 ~> 0xffffffffffffffff], [0x0 ~> 0xffffffffffffffff]]
 #[inline]
 pub fn fiat_p384_mul(out1: &mut fiat_p384_montgomery_domain_field_element, arg1: &fiat_p384_montgomery_domain_field_element, arg2: &fiat_p384_montgomery_domain_field_element) -> () {
   let x1: u64 = (arg1[1]);
@@ -851,10 +846,6 @@ pub fn fiat_p384_mul(out1: &mut fiat_p384_montgomery_domain_field_element, arg1:
 ///   eval (from_montgomery out1) mod m = (eval (from_montgomery arg1) * eval (from_montgomery arg1)) mod m
 ///   0 ≤ eval out1 < m
 ///
-/// Input Bounds:
-///   arg1: [[0x0 ~> 0xffffffffffffffff], [0x0 ~> 0xffffffffffffffff], [0x0 ~> 0xffffffffffffffff], [0x0 ~> 0xffffffffffffffff], [0x0 ~> 0xffffffffffffffff], [0x0 ~> 0xffffffffffffffff]]
-/// Output Bounds:
-///   out1: [[0x0 ~> 0xffffffffffffffff], [0x0 ~> 0xffffffffffffffff], [0x0 ~> 0xffffffffffffffff], [0x0 ~> 0xffffffffffffffff], [0x0 ~> 0xffffffffffffffff], [0x0 ~> 0xffffffffffffffff]]
 #[inline]
 pub fn fiat_p384_square(out1: &mut fiat_p384_montgomery_domain_field_element, arg1: &fiat_p384_montgomery_domain_field_element) -> () {
   let x1: u64 = (arg1[1]);
@@ -1575,11 +1566,6 @@ pub fn fiat_p384_square(out1: &mut fiat_p384_montgomery_domain_field_element, ar
 ///   eval (from_montgomery out1) mod m = (eval (from_montgomery arg1) + eval (from_montgomery arg2)) mod m
 ///   0 ≤ eval out1 < m
 ///
-/// Input Bounds:
-///   arg1: [[0x0 ~> 0xffffffffffffffff], [0x0 ~> 0xffffffffffffffff], [0x0 ~> 0xffffffffffffffff], [0x0 ~> 0xffffffffffffffff], [0x0 ~> 0xffffffffffffffff], [0x0 ~> 0xffffffffffffffff]]
-///   arg2: [[0x0 ~> 0xffffffffffffffff], [0x0 ~> 0xffffffffffffffff], [0x0 ~> 0xffffffffffffffff], [0x0 ~> 0xffffffffffffffff], [0x0 ~> 0xffffffffffffffff], [0x0 ~> 0xffffffffffffffff]]
-/// Output Bounds:
-///   out1: [[0x0 ~> 0xffffffffffffffff], [0x0 ~> 0xffffffffffffffff], [0x0 ~> 0xffffffffffffffff], [0x0 ~> 0xffffffffffffffff], [0x0 ~> 0xffffffffffffffff], [0x0 ~> 0xffffffffffffffff]]
 #[inline]
 pub fn fiat_p384_add(out1: &mut fiat_p384_montgomery_domain_field_element, arg1: &fiat_p384_montgomery_domain_field_element, arg2: &fiat_p384_montgomery_domain_field_element) -> () {
   let mut x1: u64 = 0;
@@ -1650,11 +1636,6 @@ pub fn fiat_p384_add(out1: &mut fiat_p384_montgomery_domain_field_element, arg1:
 ///   eval (from_montgomery out1) mod m = (eval (from_montgomery arg1) - eval (from_montgomery arg2)) mod m
 ///   0 ≤ eval out1 < m
 ///
-/// Input Bounds:
-///   arg1: [[0x0 ~> 0xffffffffffffffff], [0x0 ~> 0xffffffffffffffff], [0x0 ~> 0xffffffffffffffff], [0x0 ~> 0xffffffffffffffff], [0x0 ~> 0xffffffffffffffff], [0x0 ~> 0xffffffffffffffff]]
-///   arg2: [[0x0 ~> 0xffffffffffffffff], [0x0 ~> 0xffffffffffffffff], [0x0 ~> 0xffffffffffffffff], [0x0 ~> 0xffffffffffffffff], [0x0 ~> 0xffffffffffffffff], [0x0 ~> 0xffffffffffffffff]]
-/// Output Bounds:
-///   out1: [[0x0 ~> 0xffffffffffffffff], [0x0 ~> 0xffffffffffffffff], [0x0 ~> 0xffffffffffffffff], [0x0 ~> 0xffffffffffffffff], [0x0 ~> 0xffffffffffffffff], [0x0 ~> 0xffffffffffffffff]]
 #[inline]
 pub fn fiat_p384_sub(out1: &mut fiat_p384_montgomery_domain_field_element, arg1: &fiat_p384_montgomery_domain_field_element, arg2: &fiat_p384_montgomery_domain_field_element) -> () {
   let mut x1: u64 = 0;
@@ -1711,10 +1692,6 @@ pub fn fiat_p384_sub(out1: &mut fiat_p384_montgomery_domain_field_element, arg1:
 ///   eval (from_montgomery out1) mod m = -eval (from_montgomery arg1) mod m
 ///   0 ≤ eval out1 < m
 ///
-/// Input Bounds:
-///   arg1: [[0x0 ~> 0xffffffffffffffff], [0x0 ~> 0xffffffffffffffff], [0x0 ~> 0xffffffffffffffff], [0x0 ~> 0xffffffffffffffff], [0x0 ~> 0xffffffffffffffff], [0x0 ~> 0xffffffffffffffff]]
-/// Output Bounds:
-///   out1: [[0x0 ~> 0xffffffffffffffff], [0x0 ~> 0xffffffffffffffff], [0x0 ~> 0xffffffffffffffff], [0x0 ~> 0xffffffffffffffff], [0x0 ~> 0xffffffffffffffff], [0x0 ~> 0xffffffffffffffff]]
 #[inline]
 pub fn fiat_p384_opp(out1: &mut fiat_p384_montgomery_domain_field_element, arg1: &fiat_p384_montgomery_domain_field_element) -> () {
   let mut x1: u64 = 0;
@@ -1771,10 +1748,6 @@ pub fn fiat_p384_opp(out1: &mut fiat_p384_montgomery_domain_field_element, arg1:
 ///   eval out1 mod m = (eval arg1 * ((2^64)⁻¹ mod m)^6) mod m
 ///   0 ≤ eval out1 < m
 ///
-/// Input Bounds:
-///   arg1: [[0x0 ~> 0xffffffffffffffff], [0x0 ~> 0xffffffffffffffff], [0x0 ~> 0xffffffffffffffff], [0x0 ~> 0xffffffffffffffff], [0x0 ~> 0xffffffffffffffff], [0x0 ~> 0xffffffffffffffff]]
-/// Output Bounds:
-///   out1: [[0x0 ~> 0xffffffffffffffff], [0x0 ~> 0xffffffffffffffff], [0x0 ~> 0xffffffffffffffff], [0x0 ~> 0xffffffffffffffff], [0x0 ~> 0xffffffffffffffff], [0x0 ~> 0xffffffffffffffff]]
 #[inline]
 pub fn fiat_p384_from_montgomery(out1: &mut fiat_p384_non_montgomery_domain_field_element, arg1: &fiat_p384_montgomery_domain_field_element) -> () {
   let x1: u64 = (arg1[0]);
@@ -2259,10 +2232,6 @@ pub fn fiat_p384_from_montgomery(out1: &mut fiat_p384_non_montgomery_domain_fiel
 ///   eval (from_montgomery out1) mod m = eval arg1 mod m
 ///   0 ≤ eval out1 < m
 ///
-/// Input Bounds:
-///   arg1: [[0x0 ~> 0xffffffffffffffff], [0x0 ~> 0xffffffffffffffff], [0x0 ~> 0xffffffffffffffff], [0x0 ~> 0xffffffffffffffff], [0x0 ~> 0xffffffffffffffff], [0x0 ~> 0xffffffffffffffff]]
-/// Output Bounds:
-///   out1: [[0x0 ~> 0xffffffffffffffff], [0x0 ~> 0xffffffffffffffff], [0x0 ~> 0xffffffffffffffff], [0x0 ~> 0xffffffffffffffff], [0x0 ~> 0xffffffffffffffff], [0x0 ~> 0xffffffffffffffff]]
 #[inline]
 pub fn fiat_p384_to_montgomery(out1: &mut fiat_p384_montgomery_domain_field_element, arg1: &fiat_p384_non_montgomery_domain_field_element) -> () {
   let x1: u64 = (arg1[1]);
@@ -3209,8 +3178,6 @@ pub fn fiat_p384_from_bytes(out1: &mut [u64; 6], arg1: &[u8; 48]) -> () {
 ///   eval (from_montgomery out1) mod m = 1 mod m
 ///   0 ≤ eval out1 < m
 ///
-/// Output Bounds:
-///   out1: [[0x0 ~> 0xffffffffffffffff], [0x0 ~> 0xffffffffffffffff], [0x0 ~> 0xffffffffffffffff], [0x0 ~> 0xffffffffffffffff], [0x0 ~> 0xffffffffffffffff], [0x0 ~> 0xffffffffffffffff]]
 #[inline]
 pub fn fiat_p384_set_one(out1: &mut fiat_p384_montgomery_domain_field_element) -> () {
   out1[0] = 0xffffffff00000001;
