fiat-rust/src/p434_64.rs
@@ -127,11 +127,6 @@ pub fn fiat_p434_cmovznz_u64(out1: &mut u64, arg1: fiat_p434_u1, arg2: u64, arg3
 ///   eval (from_montgomery out1) mod m = (eval (from_montgomery arg1) * eval (from_montgomery arg2)) mod m
 ///   0 ≤ eval out1 < m
 ///
-/// Input Bounds:
-///   arg1: [[0x0 ~> 0xffffffffffffffff], [0x0 ~> 0xffffffffffffffff], [0x0 ~> 0xffffffffffffffff], [0x0 ~> 0xffffffffffffffff], [0x0 ~> 0xffffffffffffffff], [0x0 ~> 0xffffffffffffffff], [0x0 ~> 0xffffffffffffffff]]
-///   arg2: [[0x0 ~> 0xffffffffffffffff], [0x0 ~> 0xffffffffffffffff], [0x0 ~> 0xffffffffffffffff], [0x0 ~> 0xffffffffffffffff], [0x0 ~> 0xffffffffffffffff], [0x0 ~> 0xffffffffffffffff], [0x0 ~> 0xffffffffffffffff]]
-/// Output Bounds:
-///   out1: [[0x0 ~> 0xffffffffffffffff], [0x0 ~> 0xffffffffffffffff], [0x0 ~> 0xffffffffffffffff], [0x0 ~> 0xffffffffffffffff], [0x0 ~> 0xffffffffffffffff], [0x0 ~> 0xffffffffffffffff], [0x0 ~> 0xffffffffffffffff]]
 #[inline]
 pub fn fiat_p434_mul(out1: &mut fiat_p434_montgomery_domain_field_element, arg1: &fiat_p434_montgomery_domain_field_element, arg2: &fiat_p434_montgomery_domain_field_element) -> () {
   let x1: u64 = (arg1[1]);
@@ -1074,10 +1069,6 @@ pub fn fiat_p434_mul(out1: &mut fiat_p434_montgomery_domain_field_element, arg1:
 ///   eval (from_montgomery out1) mod m = (eval (from_montgomery arg1) * eval (from_montgomery arg1)) mod m
 ///   0 ≤ eval out1 < m
 ///
-/// Input Bounds:
-///   arg1: [[0x0 ~> 0xffffffffffffffff], [0x0 ~> 0xffffffffffffffff], [0x0 ~> 0xffffffffffffffff], [0x0 ~> 0xffffffffffffffff], [0x0 ~> 0xffffffffffffffff], [0x0 ~> 0xffffffffffffffff], [0x0 ~> 0xffffffffffffffff]]
-/// Output Bounds:
-///   out1: [[0x0 ~> 0xffffffffffffffff], [0x0 ~> 0xffffffffffffffff], [0x0 ~> 0xffffffffffffffff], [0x0 ~> 0xffffffffffffffff], [0x0 ~> 0xffffffffffffffff], [0x0 ~> 0xffffffffffffffff], [0x0 ~> 0xffffffffffffffff]]
 #[inline]
 pub fn fiat_p434_square(out1: &mut fiat_p434_montgomery_domain_field_element, arg1: &fiat_p434_montgomery_domain_field_element) -> () {
   let x1: u64 = (arg1[1]);
@@ -2021,11 +2012,6 @@ pub fn fiat_p434_square(out1: &mut fiat_p434_montgomery_domain_field_element, ar
 ///   eval (from_montgomery out1) mod m = (eval (from_montgomery arg1) + eval (from_montgomery arg2)) mod m
 ///   0 ≤ eval out1 < m
 ///
-/// Input Bounds:
-///   arg1: [[0x0 ~> 0xffffffffffffffff], [0x0 ~> 0xffffffffffffffff], [0x0 ~> 0xffffffffffffffff], [0x0 ~> 0xffffffffffffffff], [0x0 ~> 0xffffffffffffffff], [0x0 ~> 0xffffffffffffffff], [0x0 ~> 0xffffffffffffffff]]
-///   arg2: [[0x0 ~> 0xffffffffffffffff], [0x0 ~> 0xffffffffffffffff], [0x0 ~> 0xffffffffffffffff], [0x0 ~> 0xffffffffffffffff], [0x0 ~> 0xffffffffffffffff], [0x0 ~> 0xffffffffffffffff], [0x0 ~> 0xffffffffffffffff]]
-/// Output Bounds:
-///   out1: [[0x0 ~> 0xffffffffffffffff], [0x0 ~> 0xffffffffffffffff], [0x0 ~> 0xffffffffffffffff], [0x0 ~> 0xffffffffffffffff], [0x0 ~> 0xffffffffffffffff], [0x0 ~> 0xffffffffffffffff], [0x0 ~> 0xffffffffffffffff]]
 #[inline]
 pub fn fiat_p434_add(out1: &mut fiat_p434_montgomery_domain_field_element, arg1: &fiat_p434_montgomery_domain_field_element, arg2: &fiat_p434_montgomery_domain_field_element) -> () {
   let mut x1: u64 = 0;
@@ -2105,11 +2091,6 @@ pub fn fiat_p434_add(out1: &mut fiat_p434_montgomery_domain_field_element, arg1:
 ///   eval (from_montgomery out1) mod m = (eval (from_montgomery arg1) - eval (from_montgomery arg2)) mod m
 ///   0 ≤ eval out1 < m
 ///
-/// Input Bounds:
-///   arg1: [[0x0 ~> 0xffffffffffffffff], [0x0 ~> 0xffffffffffffffff], [0x0 ~> 0xffffffffffffffff], [0x0 ~> 0xffffffffffffffff], [0x0 ~> 0xffffffffffffffff], [0x0 ~> 0xffffffffffffffff], [0x0 ~> 0xffffffffffffffff]]
-///   arg2: [[0x0 ~> 0xffffffffffffffff], [0x0 ~> 0xffffffffffffffff], [0x0 ~> 0xffffffffffffffff], [0x0 ~> 0xffffffffffffffff], [0x0 ~> 0xffffffffffffffff], [0x0 ~> 0xffffffffffffffff], [0x0 ~> 0xffffffffffffffff]]
-/// Output Bounds:
-///   out1: [[0x0 ~> 0xffffffffffffffff], [0x0 ~> 0xffffffffffffffff], [0x0 ~> 0xffffffffffffffff], [0x0 ~> 0xffffffffffffffff], [0x0 ~> 0xffffffffffffffff], [0x0 ~> 0xffffffffffffffff], [0x0 ~> 0xffffffffffffffff]]
 #[inline]
 pub fn fiat_p434_sub(out1: &mut fiat_p434_montgomery_domain_field_element, arg1: &fiat_p434_montgomery_domain_field_element, arg2: &fiat_p434_montgomery_domain_field_element) -> () {
   let mut x1: u64 = 0;
@@ -2173,10 +2154,6 @@ pub fn fiat_p434_sub(out1: &mut fiat_p434_montgomery_domain_field_element, arg1:
 ///   eval (from_montgomery out1) mod m = -eval (from_montgomery arg1) mod m
 ///   0 ≤ eval out1 < m
 ///
-/// Input Bounds:
-///   arg1: [[0x0 ~> 0xffffffffffffffff], [0x0 ~> 0xffffffffffffffff], [0x0 ~> 0xffffffffffffffff], [0x0 ~> 0xffffffffffffffff], [0x0 ~> 0xffffffffffffffff], [0x0 ~> 0xffffffffffffffff], [0x0 ~> 0xffffffffffffffff]]
-/// Output Bounds:
-///   out1: [[0x0 ~> 0xffffffffffffffff], [0x0 ~> 0xffffffffffffffff], [0x0 ~> 0xffffffffffffffff], [0x0 ~> 0xffffffffffffffff], [0x0 ~> 0xffffffffffffffff], [0x0 ~> 0xffffffffffffffff], [0x0 ~> 0xffffffffffffffff]]
 #[inline]
 pub fn fiat_p434_opp(out1: &mut fiat_p434_montgomery_domain_field_element, arg1: &fiat_p434_montgomery_domain_field_element) -> () {
   let mut x1: u64 = 0;
@@ -2240,10 +2217,6 @@ pub fn fiat_p434_opp(out1: &mut fiat_p434_montgomery_domain_field_element, arg1:
 ///   eval out1 mod m = (eval arg1 * ((2^64)⁻¹ mod m)^7) mod m
 ///   0 ≤ eval out1 < m
 ///
-/// Input Bounds:
-///   arg1: [[0x0 ~> 0xffffffffffffffff], [0x0 ~> 0xffffffffffffffff], [0x0 ~> 0xffffffffffffffff], [0x0 ~> 0xffffffffffffffff], [0x0 ~> 0xffffffffffffffff], [0x0 ~> 0xffffffffffffffff], [0x0 ~> 0xffffffffffffffff]]
-/// Output Bounds:
-///   out1: [[0x0 ~> 0xffffffffffffffff], [0x0 ~> 0xffffffffffffffff], [0x0 ~> 0xffffffffffffffff], [0x0 ~> 0xffffffffffffffff], [0x0 ~> 0xffffffffffffffff], [0x0 ~> 0xffffffffffffffff], [0x0 ~> 0xffffffffffffffff]]
 #[inline]
 pub fn fiat_p434_from_montgomery(out1: &mut fiat_p434_non_montgomery_domain_field_element, arg1: &fiat_p434_montgomery_domain_field_element) -> () {
   let x1: u64 = (arg1[0]);
@@ -2831,10 +2804,6 @@ pub fn fiat_p434_from_montgomery(out1: &mut fiat_p434_non_montgomery_domain_fiel
 ///   eval (from_montgomery out1) mod m = eval arg1 mod m
 ///   0 ≤ eval out1 < m
 ///
-/// Input Bounds:
-///   arg1: [[0x0 ~> 0xffffffffffffffff], [0x0 ~> 0xffffffffffffffff], [0x0 ~> 0xffffffffffffffff], [0x0 ~> 0xffffffffffffffff], [0x0 ~> 0xffffffffffffffff], [0x0 ~> 0xffffffffffffffff], [0x0 ~> 0xffffffffffffffff]]
-/// Output Bounds:
-///   out1: [[0x0 ~> 0xffffffffffffffff], [0x0 ~> 0xffffffffffffffff], [0x0 ~> 0xffffffffffffffff], [0x0 ~> 0xffffffffffffffff], [0x0 ~> 0xffffffffffffffff], [0x0 ~> 0xffffffffffffffff], [0x0 ~> 0xffffffffffffffff]]
 #[inline]
 pub fn fiat_p434_to_montgomery(out1: &mut fiat_p434_montgomery_domain_field_element, arg1: &fiat_p434_non_montgomery_domain_field_element) -> () {
   let x1: u64 = (arg1[1]);
@@ -4069,8 +4038,6 @@ pub fn fiat_p434_from_bytes(out1: &mut [u64; 7], arg1: &[u8; 55]) -> () {
 ///   eval (from_montgomery out1) mod m = 1 mod m
 ///   0 ≤ eval out1 < m
 ///
-/// Output Bounds:
-///   out1: [[0x0 ~> 0xffffffffffffffff], [0x0 ~> 0xffffffffffffffff], [0x0 ~> 0xffffffffffffffff], [0x0 ~> 0xffffffffffffffff], [0x0 ~> 0xffffffffffffffff], [0x0 ~> 0xffffffffffffffff], [0x0 ~> 0xffffffffffffffff]]
 #[inline]
 pub fn fiat_p434_set_one(out1: &mut fiat_p434_montgomery_domain_field_element) -> () {
   out1[0] = 0x742c;
