Makefile
@@ -215,7 +215,7 @@ JAVA_$(call JAVA_RENAME,$(1))_FUNCTIONS:=$(6)
 
 endef
 
-UNSATURATED_SOLINAS_FUNCTIONS := carry_mul carry_square carry add sub opp selectznz to_bytes from_bytes
+UNSATURATED_SOLINAS_FUNCTIONS := carry_mul carry_square carry add sub opp selectznz to_bytes from_bytes relax
 FUNCTIONS_FOR_25519 := $(UNSATURATED_SOLINAS_FUNCTIONS) carry_scmul121666
 WORD_BY_WORD_MONTGOMERY_FUNCTIONS := mul square add sub opp from_montgomery to_montgomery nonzero selectznz to_bytes from_bytes one msat divstep divstep_precomp
 UNSATURATED_SOLINAS := src/ExtractionOCaml/unsaturated_solinas
